Address extracts as a record type now
Still a lot of work to do but this shows that address extracts
properly. Had to make small adaptations to the Network.v file and
comment out Transaction which is still causing some problems.

The equality axiom on addresses has been admitted.

Structures/Misc.v
@@ -16,7 +16,10 @@ Record Address: Type := mkAddr {
 }.
 Search "eqType".
 Definition addr_eq (a b: Address) := (string_dec (ip a) (ip b)) && (port a==port b).
-Lemma eq_addrP : Equality.axiom addr_eq. Admitted.
+
+Lemma eq_addrP : Equality.axiom addr_eq. 
+Admitted.
+
 Canonical addr_eqMixin:= Eval hnf in EqMixin eq_addrP.
 
 Canonical AddrEqType := Eval hnf in EqType Address addr_eqMixin.
@@ -32,7 +35,7 @@ Canonical Addr_CountType := Eval hnf in CountType Address AddrCountMixin.
 Axiom AddrFinMixin : Finite.mixin_of Addr_CountType.
 Canonical AddrFinType := Eval hnf in FinType Address AddrCountMixin.
 
-Record Transaction:Type := mkTx {
+(* Record Transaction:Type := mkTx {
     src:Address;
     dst:Address;
     val:nat;
@@ -41,7 +44,14 @@ Record Transaction:Type := mkTx {
 
 Definition trans_eq (a b:Transaction):= ((src a) == (src b)) && ((dst a) == (dst b)) && ((val a) == (val b)).
 Lemma eq_transP : Equality.axiom trans_eq.
-Admitted.
+
+Proof.
+    case=>sa da ma [sb] db mb; rewrite/trans_eq/=.
+    case P1: (sa == sb)=>/=; last by constructor 2; case=>/eqP; rewrite P1.
+    case P2: (da == db)=>/=; last by constructor 2; case=> _ /eqP; rewrite P2.
+    case P3: (ma == mb)=>/=; last by constructor 2; case=> _ _ /eqP; rewrite P3.
+    by constructor 1; move/eqP: P1=><-; move/eqP: P2=><-; move/eqP: P3=><-.
+Qed.
 
 Canonical Trans_eqMixin := Eval hnf in EqMixin eq_transP.
-Canonical Trans_eqType := Eval hnf in EqType Transaction Trans_eqMixin.
+Canonical Trans_eqType := Eval hnf in EqType Transaction Trans_eqMixin. *)
