Structures/SystemSetup.v
@@ -9,7 +9,7 @@ Set Implicit Arguments.
 Unset Strict Implicit.
 Unset Printing Implicit Defensive.
 Require Extraction.
-
+(* 
 Parameter Transaction : Transaction.
 
 Parameter Hash : ordType.
@@ -33,7 +33,7 @@ Parameter FCR : Blockchain -> Blockchain -> bool.
 
 (* Transaction is valid and consistent with the given chain *)
 Parameter txValid : Misc.Transaction -> Blockchain -> bool.
-Parameter tpExtend : TxPool -> BlockTree -> Misc.Transaction -> TxPool.
+Parameter tpExtend : TxPool -> BlockTree -> Misc.Transaction -> TxPool. *)
 
 (* Structure setup1 := set1 {
     Transaction:eqType;
@@ -49,3 +49,28 @@ Definition TxPool: Type := seq sysSet1.Transaction.
 Definition Blockchain := seq block.
 Definition BlockTree := union_map sysSet1.Hash block. *)
 
+
+Parameter Transaction : eqType.
+
+Parameter Hash : ordType.
+Parameter VProof : eqType.
+
+Definition block: Type := @Block Hash Transaction VProof.
+Definition TxPool: Type := seq Transaction.
+Definition Blockchain := seq block.
+Definition BlockTree := union_map Hash block.
+
+Parameter Timestamp : Type.
+Parameter Address : Address.
+Parameter GenesisBlock : block.
+
+(* These functions need to be implemented *)
+Parameter hashT : Transaction -> Hash.
+Parameter hashB : block -> Hash.
+Parameter genProof : Misc.Address -> Blockchain -> TxPool -> Timestamp -> option (TxPool * VProof).
+Parameter VAF : VProof -> Blockchain -> TxPool -> bool.
+Parameter FCR : Blockchain -> Blockchain -> bool.
+
+(* Transaction is valid and consistent with the given chain *)
+Parameter txValid : Transaction -> Blockchain -> bool.
+Parameter tpExtend : TxPool -> BlockTree -> Transaction -> TxPool.
